src/Distributions/UniformPowerOfTwo/Correctness.dfy
@@ -27,12 +27,14 @@ module UniformPowerOfTwo.Correctness {
   ************/
 
   ghost predicate UnifIsCorrect(n: nat, k: nat, m: nat)
-    requires (n == 0 && k == 0) || (k != 0 && Helper.Power(2, k - 1) <= n < Helper.Power(2, k))
+    requires Helper.Power(2, k) <= n < Helper.Power(2, k + 1)
   {
     RandomNumberGenerator.mu(iset s | Model.Sample(n)(s).0 == m) == if m < Helper.Power(2, k) then 1.0 / (Helper.Power(2, k) as real) else 0.0
   }
 
-  function Sample1(n: nat): RandomNumberGenerator.RNG -> RandomNumberGenerator.RNG {
+  function Sample1(n: nat): RandomNumberGenerator.RNG -> RandomNumberGenerator.RNG
+    requires n >= 1
+  {
     (s: RandomNumberGenerator.RNG) => Model.Sample(n)(s).1
   }
 
@@ -44,13 +46,14 @@ module UniformPowerOfTwo.Correctness {
   // In contrast to UnifCorrectness, this lemma does not follow
   // the thesis, but models PROB_BERN_UNIF of the HOL implementation.
   lemma UnifCorrectness2(n: nat, m: nat)
+    requires n >= 1
     ensures
       var e := iset s | Model.Sample(n)(s).0 == m;
       && e in RandomNumberGenerator.event_space
-      && RandomNumberGenerator.mu(e) == if m < Helper.Power(2, Helper.Log2(n)) then 1.0 / (Helper.Power(2, Helper.Log2(n)) as real) else 0.0
+      && RandomNumberGenerator.mu(e) == if m < Helper.Power(2, Helper.Log2Floor(n)) then 1.0 / (Helper.Power(2, Helper.Log2Floor(n)) as real) else 0.0
   {
     var e := iset s | Model.Sample(n)(s).0 == m;
-    var k := Helper.Log2(n);
+    var k := Helper.Log2Floor(n);
 
     assert e in RandomNumberGenerator.event_space by {
       assert iset{m} in MeasureTheory.natEventSpace;
@@ -63,26 +66,19 @@ module UniformPowerOfTwo.Correctness {
       }
       assert e == preimage;
     }
-
-    if k == 0 {
-      assert n == 0;
-      UnifCorrectness(n, k);
-      assert UnifIsCorrect(n, k, m);
-    } else {
-      assert n != 0;
-      Helper.Log2BothSides(n);
-      UnifCorrectness(n, k);
-      assert UnifIsCorrect(n, k, m);
-    }
+    Helper.Power2OfLog2Floor(n);
+    UnifCorrectness(n, k);
+    assert UnifIsCorrect(n, k, m);
   }
 
   // See PROB_BERN_UNIF_LT in HOL implementation.
   lemma UnifCorrectness2Inequality(n: nat, m: nat)
-    requires m <= Helper.Power(2, Helper.Log2(n))
+    requires n >= 1
+    requires m <= Helper.Power(2, Helper.Log2Floor(n))
     ensures
       var e := iset s | Model.Sample(n)(s).0 < m;
       && e in RandomNumberGenerator.event_space
-      && RandomNumberGenerator.mu(e) == (m as real) / (Helper.Power(2, Helper.Log2(n)) as real)
+      && RandomNumberGenerator.mu(e) == (m as real) / (Helper.Power(2, Helper.Log2Floor(n)) as real)
   {
     var e := iset s | Model.Sample(n)(s).0 < m;
 
@@ -110,11 +106,11 @@ module UniformPowerOfTwo.Correctness {
         { assert e1 * e2 == iset{}; RandomNumberGenerator.RNGHasMeasure(); MeasureTheory.PosCountAddImpliesAdd(RandomNumberGenerator.event_space, RandomNumberGenerator.sample_space, RandomNumberGenerator.mu); assert MeasureTheory.IsAdditive(RandomNumberGenerator.event_space, RandomNumberGenerator.mu); }
         RandomNumberGenerator.mu(e1) + RandomNumberGenerator.mu(e2);
         { UnifCorrectness2(n, m-1); UnifCorrectness2Inequality(n, m-1); }
-        (1.0 / (Helper.Power(2, Helper.Log2(n)) as real)) + (((m-1) as real) / (Helper.Power(2, Helper.Log2(n)) as real));
-        { Helper.AdditionOfFractions(1.0, (m-1) as real, Helper.Power(2, Helper.Log2(n)) as real); }
-        (1.0 + (m-1) as real) / (Helper.Power(2, Helper.Log2(n)) as real);
+        (1.0 / (Helper.Power(2, Helper.Log2Floor(n)) as real)) + (((m-1) as real) / (Helper.Power(2, Helper.Log2Floor(n)) as real));
+        { Helper.AdditionOfFractions(1.0, (m-1) as real, Helper.Power(2, Helper.Log2Floor(n)) as real); }
+        (1.0 + (m-1) as real) / (Helper.Power(2, Helper.Log2Floor(n)) as real);
         { assert 1.0 + (m-1) as real == (m as real); }
-        (m as real) / (Helper.Power(2, Helper.Log2(n)) as real);
+        (m as real) / (Helper.Power(2, Helper.Log2Floor(n)) as real);
       }
     }
   }
@@ -123,227 +119,59 @@ module UniformPowerOfTwo.Correctness {
   // In contrast to UnifCorrectness2, this lemma follows equation (4.8)
   // instead of the HOL implementation.
   lemma UnifCorrectness(n: nat, k: nat)
-    requires (n == 0 && k == 0) || (k != 0 && Helper.Power(2, k - 1) <= n < Helper.Power(2, k))
+    requires Helper.Power(2, k) <= n < Helper.Power(2, k + 1)
     ensures forall m: nat :: UnifIsCorrect(n, k, m)
   {
     forall m: nat ensures UnifIsCorrect(n, k, m) {
-      if (n == 0 && k == 0) {
-        UnifCorrectnessCaseNZeroKZero(m);
-      } else {
-        assert (k != 0 && Helper.Power(2, k - 1) <= n < Helper.Power(2, k));
-        assert n > 0;
-        assert n > 1 ==> n / 2 > 0;
-        if k - 2 < 0 {
-          assert 0 < k < 2;
-          assert k == 1;
-          assert Helper.Power(2, k) == 2;
-          assert 0 < n < 2;
-          assert n == 1;
-          assert n / 2 == 0;
-          if m % 2 == 0 {
-            UnifCorrectnessCaseKOneMEven(n, m);
-          } else {
-            assert m % 2 == 1;
-            UnifCorrectnessCaseKOneMOdd(n, m);
-          }
+      assert n >= 1 by { Helper.PowerGreater0(2, k); }
+      if k == 0 {
+        if m == 0 {
+          assert (iset s | Model.Sample(1)(s).0 == m) == (iset s);
         } else {
-          assert Helper.Power(2, k - 1) / 2 <= n / 2 < Helper.Power(2, k) / 2;
-          assert Helper.Power(2, k - 2) <= n / 2 < Helper.Power(2, k - 1);
-          var u := m / 2;
-          if m % 2 == 0 {
-            UnifCorrectnessCaseKGreaterOneMEven(n, k, m);
-          } else {
-            UnifCorrectnessCaseKGreaterOneMOdd(n, k, m);
+          assert (iset s | Model.Sample(1)(s).0 == m) == iset{};
+        }
+        RandomNumberGenerator.RNGHasMeasure();
+        assert UnifIsCorrect(n, k, m);
+      } else {
+        var u := m / 2;
+        assert Recursive: RandomNumberGenerator.mu(iset s | Model.Sample(n)(s).0 == m) == RandomNumberGenerator.mu(iset s | Model.Sample(n / 2)(s).0 == m / 2) / 2.0 by {
+          SampleProbRecursiveHalf(n, m);
+        }
+        if m < Helper.Power(2, k) {
+          assert RandomNumberGenerator.mu(iset s | Model.Sample(n / 2)(s).0 == u) == 1.0 / (Helper.Power(2, k - 1) as real) by {
+            assert u < Helper.Power(2, k - 1);
+            UnifCorrectness(n / 2, k - 1);
+            assert UnifIsCorrect(n / 2, k - 1, u);
           }
+          calc {
+            RandomNumberGenerator.mu(iset s | Model.Sample(n)(s).0 == m);
+          == { reveal Recursive; }
+            RandomNumberGenerator.mu(iset s | Model.Sample(n / 2)(s).0 == u) / 2.0;
+          ==
+            (1.0 / Helper.Power(2, k - 1) as real) / 2.0;
+          == { Helper.PowerOfTwoLemma(k - 1); }
+            1.0 / (Helper.Power(2, k) as real);
+          }
+          assert UnifIsCorrect(n, k, m);
+        } else {
+          assert u >= Helper.Power(2, k - 1);
+          reveal Recursive;
+          UnifCorrectness(n / 2, k - 1);
+          assert UnifIsCorrect(n / 2, k - 1, u);
+          assert RandomNumberGenerator.mu(iset s | Model.Sample(n)(s).0 == m) == 0.0;
         }
       }
     }
   }
 
-  lemma UnifCorrectnessCaseNZeroKZero(m: nat)
-    ensures UnifIsCorrect(0, 0, m)
-  {
-    assert Helper.Power(2, 0) == 1;
-    if m == 0 {
-      assert (iset s | Model.Sample(0)(s).0 == m) == (iset s | true);
-      RandomNumberGenerator.RNGHasMeasure();
-    } else {
-      assert (iset s | Model.Sample(0)(s).0 == m) == iset{};
-      RandomNumberGenerator.RNGHasMeasure();
-    }
-  }
-
-  lemma UnifCorrectnessCaseKOneMEven(n: nat, m: nat)
-    requires 1 <= n < 2
-    requires m % 2 == 0
-    ensures UnifIsCorrect(n, 1, m)
-  {
-    calc {
-      RandomNumberGenerator.mu(iset s | Model.Sample(n)(s).0 == m);
-    == { SampleCaseSplit(n, m); }
-      RandomNumberGenerator.mu(iset s | 2*Model.Sample(n / 2)(s).0 == m) / 2.0;
-    == { assert (iset s | 2*Model.Sample(n / 2)(s).0 == m) == (iset s | 0 == m); }
-      RandomNumberGenerator.mu(iset s | 0 == m) / 2.0;
-    }
-    if m < Helper.Power(2, 1) {
-      assert m == 0;
-      calc {
-        RandomNumberGenerator.mu(iset s | Model.Sample(n)(s).0 == m);
-      ==
-        RandomNumberGenerator.mu(iset s | 0 == m) / 2.0;
-      == { assert (iset s: RandomNumberGenerator.RNG | 0 == m) == (iset s | true); }
-        RandomNumberGenerator.mu(iset s | true) / 2.0;
-      == { RandomNumberGenerator.RNGHasMeasure(); }
-        1.0 / 2.0;
-      ==
-        1.0 / (2 as real);
-      == { assert Helper.Power(2, 1) == 2; }
-        1.0 / (Helper.Power(2, 1) as real);
-      }
-    } else {
-      assert m != 0;
-      calc {
-        RandomNumberGenerator.mu(iset s | Model.Sample(n)(s).0 == m);
-      ==
-        RandomNumberGenerator.mu(iset s | 0 == m) / 2.0;
-      == { assert (iset s: RandomNumberGenerator.RNG | 0 == m) == iset{}; }
-        RandomNumberGenerator.mu(iset {}) / 2.0;
-      == { RandomNumberGenerator.RNGHasMeasure(); }
-        0.0 / 2.0;
-      ==
-        0.0;
-      }
-    }
-  }
-
-  lemma UnifCorrectnessCaseKOneMOdd(n: nat, m: nat)
-    requires 1 <= n < 2
-    requires m % 2 == 1
-    ensures UnifIsCorrect(n, 1, m)
-  {
-    calc {
-      RandomNumberGenerator.mu(iset s | Model.Sample(n)(s).0 == m);
-    == { SampleCaseSplit(n, m); }
-      RandomNumberGenerator.mu(iset s | 2*Model.Sample(n / 2)(s).0 + 1 == m) / 2.0;
-    == { assert (iset s | 2*Model.Sample(n / 2)(s).0 + 1 == m) == (iset s | 1 == m); }
-      RandomNumberGenerator.mu(iset s | 1 == m) / 2.0;
-    }
-    if m < Helper.Power(2, 1) {
-      assert m == 1;
-      calc {
-        RandomNumberGenerator.mu(iset s | Model.Sample(n)(s).0 == m);
-      ==
-        RandomNumberGenerator.mu(iset s | 1 == m) / 2.0;
-      == { assert (iset s: RandomNumberGenerator.RNG | 1 == m) == (iset s | true); }
-        RandomNumberGenerator.mu(iset s | true) / 2.0;
-      == { RandomNumberGenerator.RNGHasMeasure(); Helper.DivisionSubstituteAlternativeReal(2.0, RandomNumberGenerator.mu(iset s | true), 1.0); }
-        1.0 / 2.0;
-      ==
-        1.0 / (Helper.Power(2, 1) as real);
-      }
-    } else {
-      assert m != 1;
-      calc {
-        RandomNumberGenerator.mu(iset s: RandomNumberGenerator.RNG | Model.Sample(n)(s).0 == m);
-      ==
-        RandomNumberGenerator.mu(iset s: RandomNumberGenerator.RNG | 1 == m) / 2.0;
-      == { assert (iset s: RandomNumberGenerator.RNG | 1 == m) == iset{}; }
-        RandomNumberGenerator.mu(iset {}) / 2.0;
-      == { RandomNumberGenerator.RNGHasMeasure(); }
-        0.0 / 2.0;
-      ==
-        0.0;
-      }
-    }
-  }
-
-  lemma UnifCorrectnessCaseKGreaterOneMEven(n: nat, k: nat, m: nat)
-    requires k >= 2
-    requires Helper.Power(2, k - 1) <= n < Helper.Power(2, k)
-    requires m % 2 == 0
-    ensures UnifIsCorrect(n, k, m)
-  {
-    var u := m / 2;
-    assert m == 2 * u;
-    calc {
-      RandomNumberGenerator.mu(iset s | Model.Sample(n)(s).0 == m);
-    == { SampleCaseSplit(n, m); }
-      RandomNumberGenerator.mu(iset s | 2 * Model.Sample(n / 2)(s).0 == m) / 2.0;
-    == { assert (iset s | 2 * Model.Sample(n / 2)(s).0 == m) == (iset s | Model.Sample(n / 2)(s).0 == u); }
-      RandomNumberGenerator.mu(iset s | Model.Sample(n / 2)(s).0 == u) / 2.0;
-    }
-    if m < Helper.Power(2, k) {
-      assert RandomNumberGenerator.mu(iset s | Model.Sample(n / 2)(s).0 == u) == 1.0 / (Helper.Power(2, k - 1) as real) by {
-        assert u < Helper.Power(2, k - 1);
-        UnifCorrectness(n / 2, k - 1);
-        assert UnifIsCorrect(n / 2, k - 1, u);
-      }
-      calc {
-        RandomNumberGenerator.mu(iset s | Model.Sample(n)(s).0 == m);
-      ==
-        RandomNumberGenerator.mu(iset s | Model.Sample(n / 2)(s).0 == u) / 2.0;
-      ==
-        (1.0 / Helper.Power(2, k - 1) as real) / 2.0;
-      == { Helper.PowerOfTwoLemma(k - 1); }
-        1.0 / (Helper.Power(2, k) as real);
-      }
-      assert UnifIsCorrect(n / 2, k - 1, u);
-    } else {
-      assert u >= Helper.Power(2, k - 1);
-      UnifCorrectness(n / 2, k - 1);
-      assert UnifIsCorrect(n / 2, k - 1, u);
-      assert RandomNumberGenerator.mu(iset s | Model.Sample(n)(s).0 == m) == 0.0;
-      assert UnifIsCorrect(n / 2, k - 1, u);
-    }
-  }
-
-  lemma UnifCorrectnessCaseKGreaterOneMOdd(n: nat, k: nat, m: nat)
-    requires k >= 2
-    requires Helper.Power(2, k - 1) <= n < Helper.Power(2, k)
-    requires m % 2 == 1
-    ensures UnifIsCorrect(n, k, m)
-  {
-    var u := m / 2;
-    assert m == 2 * u + 1;
-    calc {
-      RandomNumberGenerator.mu(iset s | Model.Sample(n)(s).0 == m);
-    == { SampleCaseSplit(n, m); }
-      RandomNumberGenerator.mu(iset s | 2 * Model.Sample(n / 2)(s).0 + 1 == m) / 2.0;
-    == { assert (iset s | 2 * Model.Sample(n / 2)(s).0 + 1 == m) == (iset s | Model.Sample(n / 2)(s).0 == u); }
-      RandomNumberGenerator.mu(iset s | Model.Sample(n / 2)(s).0 == u) / 2.0;
-    }
-    if m < Helper.Power(2, k) {
-      assert RandomNumberGenerator.mu(iset s | Model.Sample(n / 2)(s).0 == u) == 1.0 / (Helper.Power(2, k - 1) as real) by {
-        assert u < Helper.Power(2, k - 1);
-        UnifCorrectness(n / 2, k - 1);
-        assert UnifIsCorrect(n / 2, k - 1, u);
-      }
-      calc {
-        RandomNumberGenerator.mu(iset s | Model.Sample(n)(s).0 == m);
-      ==
-        RandomNumberGenerator.mu(iset s | Model.Sample(n / 2)(s).0 == u) / 2.0;
-      ==
-        (1.0 / Helper.Power(2, k - 1) as real) / 2.0;
-      == { Helper.PowerOfTwoLemma(k - 1); }
-        1.0 / (Helper.Power(2, k) as real);
-      }
-      assert UnifIsCorrect(n, k, m);
-    } else {
-      assert u >= Helper.Power(2, k - 1);
-      UnifCorrectness(n / 2, k - 1);
-      assert UnifIsCorrect(n / 2, k - 1, u);
-      assert RandomNumberGenerator.mu(iset s | Model.Sample(n)(s).0 == m) == 0.0;
-      assert UnifIsCorrect(n, k, m);
-    }
-  }
-
   // Equation (4.7)
   lemma SampleIsIndepFn(n: nat)
+    requires n >= 1
     decreases n
     ensures Independence.IsIndepFn(Model.Sample(n))
   {
     var fn := Model.Sample(n);
-    if n == 0 {
+    if n == 1 {
       Independence.ReturnIsIndepFn(0 as nat);
     } else {
       assert Independence.IsIndepFn(Model.Sample(n / 2)) by {
@@ -362,6 +190,7 @@ module UniformPowerOfTwo.Correctness {
   }
 
   lemma SampleIsMeasurePreserving(n: nat)
+    requires n >= 1
     ensures MeasureTheory.IsMeasurePreserving(RandomNumberGenerator.event_space, RandomNumberGenerator.mu, RandomNumberGenerator.event_space, RandomNumberGenerator.mu, Sample1(n))
   {
     var f := Sample1(n);
@@ -370,8 +199,7 @@ module UniformPowerOfTwo.Correctness {
       Independence.IsIndepFnImpliesSndMeasurable(Model.Sample(n));
       assert Independence.IsIndepFn(Model.Sample(n));
     }
-    var g := Sample1(n / 2);
-    if n == 0 {
+    if n == 1 {
       forall e | e in RandomNumberGenerator.event_space ensures RandomNumberGenerator.mu(MeasureTheory.PreImage(f, e)) == RandomNumberGenerator.mu(e) {
         forall s: RandomNumberGenerator.RNG ensures f(s) == s {
           assert f(s) == s;
@@ -380,6 +208,7 @@ module UniformPowerOfTwo.Correctness {
       }
       assert MeasureTheory.IsMeasurePreserving(RandomNumberGenerator.event_space, RandomNumberGenerator.mu, RandomNumberGenerator.event_space, RandomNumberGenerator.mu, f);
     } else {
+      var g := Sample1(n / 2);
       forall e | e in RandomNumberGenerator.event_space ensures RandomNumberGenerator.mu(MeasureTheory.PreImage(f, e)) == RandomNumberGenerator.mu(e) {
         var e' := (iset s | Monad.Tail(s) in e);
         assert e' in RandomNumberGenerator.event_space by {
@@ -424,7 +253,7 @@ module UniformPowerOfTwo.Correctness {
   }
 
   lemma SampleTailDecompose(n: nat, s: RandomNumberGenerator.RNG)
-    requires n != 0
+    requires n >= 2
     ensures Model.Sample(n)(s).1 == Monad.Tail(Model.Sample(n / 2)(s).1)
   {
     var (a, s') := Model.Sample(n / 2)(s);
@@ -448,244 +277,67 @@ module UniformPowerOfTwo.Correctness {
     }
   }
 
-  lemma SampleCorrectnessIff(n: nat, s: RandomNumberGenerator.RNG, m: nat)
-    requires n > 0
-    ensures
-      var a := Model.Sample(n / 2)(s).0;
-      var b := Monad.Deconstruct(Model.Sample(n / 2)(s).1).0;
-      Model.Sample(n)(s).0 == m
-      <==>
-      (b && 2*a + 1 == m) || (!b && 2*a == m)
-  {
-    var (a, s') := Model.Sample(n / 2)(s);
-    var (b, s'') := Monad.Deconstruct(s');
-    calc {
-      Model.Sample(n)(s).0;
-    ==
-      Monad.Bind(Model.Sample(n / 2), Model.UnifStep)(s).0;
-    ==
-      Model.UnifStep(a)(s').0;
-    ==
-      Monad.Bind(Monad.Deconstruct, b => Monad.Return(if b then 2*a + 1 else 2*a))(s').0;
-    ==
-      Monad.Return(if b then 2*a + 1 else 2*a)(s'').0;
-    ==
-      if b then 2*a + 1 else 2*a;
-    }
-  }
-
-  lemma SampleCorrectnessEvenCaseIff(n: nat, s: RandomNumberGenerator.RNG, m: nat)
-    requires m % 2 == 0
-    requires n > 0
-    ensures
-      var a := Model.Sample(n / 2)(s).0;
-      var b := Monad.Deconstruct(Model.Sample(n / 2)(s).1).0;
-      Model.Sample(n)(s).0 == m <==> (!b && 2*a == m)
-  {
-    var a: nat := Model.Sample(n / 2)(s).0;
-    var b := Monad.Deconstruct(Model.Sample(n / 2)(s).1).0;
-    if Model.Sample(n)(s).0 == m {
-      if (b && 2*a + 1 == m) {
-        assert m % 2 == 1 by {
-          Helper.DivModAddMultiple(2, 1, a);
-        }
-        assert m % 2 == 0;
-        assert false;
-      }
-      assert !(b && 2*a + 1 == m) ==> (!b && 2*a == m) by {
-        SampleCorrectnessIff(n, s, m);
-        assert (b && 2*a + 1 == m) || (!b && 2*a == m);
-      }
-    }
-    if (!b && 2*a == m) {
-      assert (b && 2*a + 1 == m) || (!b && 2*a == m);
-      assert Model.Sample(n)(s).0 == m by { SampleCorrectnessIff(n, s, m); }
-    }
-  }
-
-  lemma SampleOddCaseIff(n: nat, s: RandomNumberGenerator.RNG, m: nat)
-    requires m % 2 == 1
-    requires n > 0
-    ensures
-      var a := Model.Sample(n / 2)(s).0;
-      var b := Monad.Deconstruct(Model.Sample(n / 2)(s).1).0;
-      Model.Sample(n)(s).0 == m <==> (b && 2*a + 1 == m)
-  {
-    var a := Model.Sample(n / 2)(s).0;
-    var b := Monad.Deconstruct(Model.Sample(n / 2)(s).1).0;
-    if Model.Sample(n)(s).0 == m {
-      if (!b && 2*a == m) {
-        assert m % 2 == 0 by { assert m / 2 == a; }
-        assert m % 2 == 1;
-      }
-      assert !(!b && 2*a == m) ==> (b && 2*a + 1 == m) by {
-        SampleCorrectnessIff(n, s, m);
-        assert (b && 2*a + 1 == m) || (!b && 2*a == m);
-      }
-    }
-    if (b && 2*a + 1 == m) {
-      assert (b && 2*a + 1 == m) || (!b && 2*a == m);
-      assert Model.Sample(n)(s).0 == m by { SampleCorrectnessIff(n, s, m); }
-    }
-  }
-
-  lemma SampleEvenCaseSetEquality(n: nat, m: nat)
-    requires m % 2 == 0
-    requires n > 0
+  lemma SampleSetEquality(n: nat, m: nat)
+    requires n >= 2
     ensures
       var b_of := (s: RandomNumberGenerator.RNG) => Monad.Deconstruct(Model.Sample(n / 2)(s).1).0;
       var a_of := (s: RandomNumberGenerator.RNG) => Model.Sample(n / 2)(s).0;
-      (iset s | Model.Sample(n)(s).0 == m) == (iset s | !b_of(s) && 2*a_of(s) == m)
+      (iset s | Model.Sample(n)(s).0 == m) == (iset s | 2*a_of(s) + (if b_of(s) then 1 else 0) == m)
   {
     var b_of := (s: RandomNumberGenerator.RNG) => Monad.Deconstruct(Model.Sample(n / 2)(s).1).0;
     var a_of := (s: RandomNumberGenerator.RNG) => Model.Sample(n / 2)(s).0;
-    forall s ensures Model.Sample(n)(s).0 == m <==> (!b_of(s) && 2*a_of(s) == m) {
-      SampleCorrectnessEvenCaseIff(n, s, m);
-    }
-  }
-
-  lemma SampleOddCaseSetEquality(n: nat, m: nat)
-    requires m % 2 == 1
-    requires n > 0
-    ensures
-      var b_of := (s: RandomNumberGenerator.RNG) => Monad.Deconstruct(Model.Sample(n / 2)(s).1).0;
-      var a_of := (s: RandomNumberGenerator.RNG) => Model.Sample(n / 2)(s).0;
-      (iset s | Model.Sample(n)(s).0 == m) == (iset s | b_of(s) && 2*a_of(s) + 1 == m)
-  {
-    var b_of := (s: RandomNumberGenerator.RNG) => Monad.Deconstruct(Model.Sample(n / 2)(s).1).0;
-    var a_of := (s: RandomNumberGenerator.RNG) => Model.Sample(n / 2)(s).0;
-    forall s ensures Model.Sample(n)(s).0 == m <==> (b_of(s) && 2*a_of(s) + 1 == m) {
-      SampleOddCaseIff(n, s, m);
-    }
-  }
-
-  lemma SampleEvenCase(n: nat, m: nat)
-    requires m % 2 == 0
-    requires n > 0
-    ensures RandomNumberGenerator.mu(iset s | Model.Sample(n)(s).0 == m) == RandomNumberGenerator.mu(iset s | 2*Model.Sample(n / 2)(s).0 == m) / 2.0
-  {
-    var a_of := (s: RandomNumberGenerator.RNG) => Model.Sample(n / 2)(s).0;
-    var b_of := (s: RandomNumberGenerator.RNG) => Monad.Deconstruct(Model.Sample(n / 2)(s).1).0;
-    var A: iset<nat> := (iset x | 2*x == m);
-    var E: iset<RandomNumberGenerator.RNG> := (iset s | Monad.Deconstruct(s).0 == false);
-    var f := Sample1(n / 2);
-
-    var e1 := (iset s | Sample1(n / 2)(s) in E);
-    var e2 := (iset s | Model.Sample(n / 2)(s).0 in A);
-
-    assert Eq1: (iset s | !b_of(s)) == e1 by {
-      forall s ensures !b_of(s) <==> Model.Sample(n / 2)(s).1 in E {
-      }
-    }
-
-    assert Eq2: (iset s | 2*a_of(s) == m) == e2 by {
-      forall s ensures 2*a_of(s) == m <==> Model.Sample(n / 2)(s).0 in A {
-      }
-    }
-
-    assert Eq3: (iset s | 2*a_of(s) == m) == (iset s | 2*Model.Sample(n / 2)(s).0 == m) by {
-      forall s ensures 2*a_of(s) == m <==> 2*Model.Sample(n / 2)(s).0 == m {
-      }
-    }
-
-    assert Eq4: e1 == MeasureTheory.PreImage(Sample1(n / 2), E) by {
-      forall s ensures Model.Sample(n / 2)(s).1 in E <==> f(s) in E {
-      }
-    }
-
-    assert EMeasure: E in RandomNumberGenerator.event_space && RandomNumberGenerator.mu(E) == 0.5 by {
-      assert E == (iset s | Monad.Head(s) == false);
-      Monad.HeadIsMeasurable(false);
-    }
-
-    assert Indep: RandomNumberGenerator.mu(e1 * e2) == RandomNumberGenerator.mu(e1) * RandomNumberGenerator.mu(e2) by {
-      assert e1 == (iset s | Model.Sample(n / 2)(s).1 in E) by {
-        forall s ensures s in e1 <==> Model.Sample(n / 2)(s).1 in E {
-        }
-      }
-      assert MeasureTheory.AreIndepEvents(RandomNumberGenerator.event_space, RandomNumberGenerator.mu, e1, e2) by {
-        assert Independence.IsIndepFunction(Model.Sample(n / 2)) by {
-          assert Independence.IsIndepFn(Model.Sample(n / 2)) by {
-            SampleIsIndepFn(n / 2);
-          }
-          Independence.IsIndepFnImpliesIsIndepFunction(Model.Sample(n / 2));
-        }
-        assert E in RandomNumberGenerator.event_space by { reveal EMeasure; }
-        assert Independence.IsIndepFunctionCondition(Model.Sample(n / 2), A, E);
-      }
-      Independence.AreIndepEventsConjunctElimination(e1, e2);
-    }
-
-    assert Prob: 0.5 == RandomNumberGenerator.mu(e1) by {
+    forall s ensures Model.Sample(n)(s).0 == m <==> (2 * a_of(s) + (if b_of(s) then 1 else 0) == m) {
+      var (a, s') := Model.Sample(n / 2)(s);
+      var (b, s'') := Monad.Deconstruct(s');
       calc {
-        0.5;
-      == { reveal EMeasure; }
-        RandomNumberGenerator.mu(E);
-      == { reveal EMeasure; SampleIsMeasurePreserving(n / 2); }
-        RandomNumberGenerator.mu(MeasureTheory.PreImage(Sample1(n / 2), E));
-      == { reveal Eq4; }
-        RandomNumberGenerator.mu(e1);
+        Model.Sample(n)(s).0;
+      ==
+        Monad.Bind(Model.Sample(n / 2), Model.UnifStep)(s).0;
+      ==
+        Model.UnifStep(a)(s').0;
+      ==
+        Monad.Bind(Monad.Deconstruct, b => Monad.Return(if b then 2*a + 1 else 2*a))(s').0;
+      ==
+        Monad.Return(if b then 2*a + 1 else 2*a)(s'').0;
+      ==
+        if b then 2*a + 1 else 2*a;
       }
-    }
-
-    assert Inter: (iset s | !b_of(s) && 2*a_of(s) == m) == (iset s | !b_of(s)) * (iset s | 2*a_of(s) == m) by {
-      forall s ensures !b_of(s) && 2*a_of(s) == m <==> !b_of(s) && 2*a_of(s) == m {
-      }
-    }
-
-    assert MulSub: RandomNumberGenerator.mu(e1) * RandomNumberGenerator.mu(e2) == 0.5 * RandomNumberGenerator.mu(e2) by {
-      reveal EMeasure;
-      assert RandomNumberGenerator.mu(e1) == 0.5 by { reveal Prob; }
-      assert RandomNumberGenerator.mu(e1) == 0.5 ==> RandomNumberGenerator.mu(e1) * RandomNumberGenerator.mu(e2) == 0.5 * RandomNumberGenerator.mu(e2);
-    }
-
-    calc {
-      RandomNumberGenerator.mu(iset s | Model.Sample(n)(s).0 == m);
-    == { SampleEvenCaseSetEquality(n, m); }
-      RandomNumberGenerator.mu(iset s | !b_of(s) && 2*a_of(s) == m);
-    == {  reveal Inter; }
-      RandomNumberGenerator.mu((iset s | !b_of(s)) * (iset s | 2*a_of(s) == m));
-    == { reveal Eq1; reveal Eq2; }
-      RandomNumberGenerator.mu(e1 * e2);
-    == { reveal Indep; }
-      RandomNumberGenerator.mu(e1) * RandomNumberGenerator.mu(e2);
-    == { reveal MulSub; }
-      0.5 * RandomNumberGenerator.mu(e2);
-    == { Helper.DivisionByTwo(RandomNumberGenerator.mu(e2)); }
-      RandomNumberGenerator.mu(e2) / 2.0;
-    == { reveal Eq2; }
-      RandomNumberGenerator.mu(iset s | 2*a_of(s) == m) / 2.0;
-    == { reveal Eq3; }
-      RandomNumberGenerator.mu(iset s | 2*Model.Sample(n / 2)(s).0 == m) / 2.0;
     }
   }
 
-  lemma SampleOddCase(n: nat, m: nat)
-    requires m % 2 == 1
-    requires n > 0
-    ensures RandomNumberGenerator.mu(iset s | Model.Sample(n)(s).0 == m) == RandomNumberGenerator.mu(iset s | 2*Model.Sample(n / 2)(s).0 + 1 == m) / 2.0
+  lemma SampleProbRecursiveHalf(n: nat, m: nat)
+    requires n >= 2
+    ensures RandomNumberGenerator.mu(iset s | Model.Sample(n)(s).0 == m) == RandomNumberGenerator.mu(iset s | Model.Sample(n / 2)(s).0 == m / 2) / 2.0
   {
     var a_of := (s: RandomNumberGenerator.RNG) => Model.Sample(n / 2)(s).0;
     var b_of := (s: RandomNumberGenerator.RNG) => Monad.Deconstruct(Model.Sample(n / 2)(s).1).0;
-    var A: iset<nat> := (iset x | 2*x + 1 == m);
-    var E: iset<RandomNumberGenerator.RNG> := (iset s | Monad.Deconstruct(s).0 == true);
+    var A: iset<nat> := (iset x | x == m / 2);
+    var E: iset<RandomNumberGenerator.RNG> := (iset s | m % 2 == if Monad.Deconstruct(s).0 then 1 else 0);
     var f := (s: RandomNumberGenerator.RNG) => Model.Sample(n / 2)(s).1;
 
     var e1 := (iset s | Model.Sample(n / 2)(s).1 in E);
     var e2 := (iset s | Model.Sample(n / 2)(s).0 in A);
+    var e3 := (iset s | 2*a_of(s) + (if b_of(s) then 1 else 0) == m);
 
-    assert Eq1: (iset s | b_of(s)) == e1 by {
-      forall s ensures b_of(s) <==> Model.Sample(n / 2)(s).1 in E {
+    assert SplitEvent: e3 == e1 * e2 by {
+      forall s ensures s in e3 <==> s in e1 && s in e2 {
+        calc {
+          s in e3;
+          2*a_of(s) + (if b_of(s) then 1 else 0) == m;
+          (m % 2 == if b_of(s) then 1 else 0) && a_of(s) == m / 2;
+          s in e1 && s in e2;
+        }
       }
     }
 
-    assert Eq2: (iset s | 2*a_of(s) + 1 == m) == e2 by {
-      forall s ensures 2*a_of(s) + 1 == m <==> Model.Sample(n / 2)(s).0 in A {
+    assert Eq2: (iset s | a_of(s) == m / 2) == e2 by {
+      forall s ensures a_of(s) == m / 2 <==> Model.Sample(n / 2)(s).0 in A {
       }
     }
 
-    assert Eq3: (iset s | 2*a_of(s) + 1 == m) == (iset s | 2*Model.Sample(n / 2)(s).0 + 1 == m) by {
-      forall s ensures 2*a_of(s) + 1 == m <==> 2*Model.Sample(n / 2)(s).0 + 1 == m {
+    assert Eq3: (iset s | a_of(s) == m / 2) == (iset s | Model.Sample(n / 2)(s).0 == m / 2) by {
+      forall s ensures a_of(s) == m / 2 <==> Model.Sample(n / 2)(s).0 == m / 2 {
+        assert a_of(s) == Model.Sample(n / 2)(s).0;
       }
     }
 
@@ -695,8 +347,8 @@ module UniformPowerOfTwo.Correctness {
     }
 
     assert E in RandomNumberGenerator.event_space && RandomNumberGenerator.mu(E) == 0.5 by {
-      assert E == (iset s | Monad.Head(s) == true);
-      Monad.HeadIsMeasurable(true);
+      assert E == (iset s | Monad.Head(s) == (m % 2 == 1));
+      Monad.HeadIsMeasurable(m % 2 == 1);
     }
 
     assert Indep: RandomNumberGenerator.mu(e1 * e2) == RandomNumberGenerator.mu(e1) * RandomNumberGenerator.mu(e2) by {
@@ -713,7 +365,7 @@ module UniformPowerOfTwo.Correctness {
       Independence.AreIndepEventsConjunctElimination(e1, e2);
     }
 
-    assert Prob: 0.5 == RandomNumberGenerator.mu(e1) by {
+    assert ProbE1: 0.5 == RandomNumberGenerator.mu(e1) by {
       calc {
         0.5;
       ==
@@ -725,40 +377,22 @@ module UniformPowerOfTwo.Correctness {
       }
     }
 
-    assert Prob2: RandomNumberGenerator.mu(e1) * RandomNumberGenerator.mu(e2) == 0.5 * RandomNumberGenerator.mu(e2) by {
-      reveal Prob;
-    }
-
     calc {
       RandomNumberGenerator.mu(iset s | Model.Sample(n)(s).0 == m);
-    == { SampleOddCaseSetEquality(n, m); }
-      RandomNumberGenerator.mu(iset s | b_of(s) && 2*a_of(s) + 1 == m);
-    == { assert (iset s | b_of(s) && 2*a_of(s) + 1 == m) == (iset s | b_of(s)) * (iset s | 2*a_of(s) + 1 == m); }
-      RandomNumberGenerator.mu((iset s | b_of(s)) * (iset s | 2*a_of(s) + 1 == m));
-    == { reveal Eq1; reveal Eq2; }
+    == { SampleSetEquality(n, m); }
+      RandomNumberGenerator.mu(e3);
+    == { reveal SplitEvent; }
       RandomNumberGenerator.mu(e1 * e2);
     == { reveal Indep; }
       RandomNumberGenerator.mu(e1) * RandomNumberGenerator.mu(e2);
-    == { reveal Prob2; }
+    == { reveal ProbE1; }
       0.5 * RandomNumberGenerator.mu(e2);
     ==
       RandomNumberGenerator.mu(e2) / 2.0;
     == { reveal Eq2; }
-      RandomNumberGenerator.mu(iset s | 2*a_of(s) + 1 == m) / 2.0;
+      RandomNumberGenerator.mu(iset s | a_of(s) == m / 2) / 2.0;
     == { reveal Eq3; }
-      RandomNumberGenerator.mu(iset s | 2*Model.Sample(n / 2)(s).0 + 1 == m) / 2.0;
+      RandomNumberGenerator.mu(iset s | Model.Sample(n / 2)(s).0 == m / 2) / 2.0;
     }
   }
-
-  lemma SampleCaseSplit(n: nat, m: nat)
-    requires n > 0
-    ensures RandomNumberGenerator.mu(iset s | Model.Sample(n)(s).0 == m) == if m % 2 == 0 then RandomNumberGenerator.mu(iset s | 2*Model.Sample(n / 2)(s).0 == m) / 2.0 else RandomNumberGenerator.mu(iset s | 2*Model.Sample(n / 2)(s).0 + 1 == m) / 2.0
-  {
-    if m % 2 == 0 {
-      SampleEvenCase(n, m);
-    } else {
-      SampleOddCase(n, m);
-    }
-  }
-
 }
